src/go_lang/struct.v
@@ -81,6 +81,13 @@ Definition structTy (d:descriptor) : ty :=
 Definition structRefTy (d:descriptor) : ty :=
   structRefT (flatten_ty (structTy d)).
 
+Fixpoint ty_size (t:ty) : Z :=
+  match t with
+  | prodT t1 t2 => ty_size t1 + ty_size t2
+  (* this gives unit values space, which seems fine *)
+  | _ => 1
+  end.
+
 Fixpoint load_ty (t:ty) (e:expr) : expr :=
   match t with
   | prodT t1 t2 => (load_ty t1 e, load_ty t2 (e +ₗ #(ty_size t1)))
@@ -177,6 +184,7 @@ Proof.
   pose proof (ty_size_gt_0 t2).
   rewrite app_length; auto.
   rewrite Z2Nat.inj_add; lia.
+
 Qed.
 
 Hint Rewrite ty_size_length : ty.
